code/Yazi.LZ77.fsti
@@ -3,9 +3,12 @@ module Yazi.LZ77
 module B = LowStar.Buffer
 module CB = LowStar.ConstBuffer
 module CFlags = Yazi.CFlags
+module I32 = FStar.Int32
 module S = Spec.LZ77
+module SST = Yazi.Stream.Types
 module ST = FStar.HyperStack.ST
 module U32 = FStar.UInt32
+module U8 = FStar.UInt8
 
 include Yazi.LZ77.Types
 
@@ -28,3 +31,16 @@ val slide_hash: ctx: lz77_context_p -> h_range: U32.t -> ST.Stack unit
   (ensures fun h0 _ h1 ->
     B.modifies (S.hash_loc_buffer h0 ctx) h0 h1 /\
     S.hash_chain_valid h1 ctx h_range true)
+
+val fill_window:
+    ss: SST.stream_state_t
+  -> ctx: lz77_context_p
+  -> ls: lz77_state_t
+  -> next_in: SST.io_buffer
+  -> wrap: SST.wrap_t
+  -> block_start: B.pointer I32.t
+  -> block_data: Ghost.erased (Seq.seq U8.t)
+  -> ST.Stack (Ghost.erased (Seq.seq U8.t))
+  (requires fun h -> S.fill_window_pre h ss ctx ls next_in wrap block_start block_data)
+  (ensures fun h0 res h1 ->
+    S.fill_window_post h0 res h1 ss ctx ls next_in wrap block_start block_data)
